code/experimental/P256/Hacl.Impl.ECDSA.P256SHA256.Verification.fst
@@ -1,0 +1,63 @@
+module Hacl.Impl.ECDSA.P256SHA256.Verification
+
+open FStar.HyperStack.All
+open FStar.HyperStack
+module ST = FStar.HyperStack.ST
+
+open Lib.IntTypes
+open Lib.Buffer
+
+open Hacl.Spec.P256.Definitions
+open Hacl.Impl.LowLevel
+open Hacl.Impl.P256
+
+open Hacl.Impl.Curve25519.Field64.Core
+
+val isCoordinateValid: p: lbuffer uint64 (size 12) -> Stack bool 
+  (requires fun h -> live h p)
+  (ensures fun h0 _ h1 -> h0 == h1 /\
+    as_nat h1 (gsub p (size 0) (size 4)) < prime /\ 
+    as_nat h1 (gsub p (size 4) (size 4)) < prime /\
+    as_nat h1 (gsub p (size 8) (size 4)) < prime
+  )
+
+
+let isCoordinateValid p = 
+  push_frame();
+    let tempBuffer = create (size 4) (u64 0) in 
+    let x = sub p (size 0) (size 4) in 
+    let y = sub p (size 4) (size 4) in 
+    let z = sub p (size 8) (size 4) in 
+    let carryX = sub4_il x prime_buffer tempBuffer in 
+    let carryY = sub4_il y prime_buffer tempBuffer in 
+    let carryZ = sub4_il z prime_buffer tempBuffer in 
+
+    let lessX = eq #U64  carryX (u64 0) in 
+    let lessY = eq #U64 carryY (u64 0) in 
+    let lessZ = eq #U64  carryZ (u64 0) in 
+
+      pop_frame()  ; 
+    lessX && lessY && lessZ
+
+
+
+val ecdsa_verification: 
+  pubKey: point -> 
+  r: lbuffer uint64 (size 4) ->
+  s: lbuffer uint64 (size 4) ->
+  mLen: size_t ->
+  m: lbuffer uint64 mLen -> 
+  tempBuffer: lbuffer uint64 (size 10000) -> 
+  Stack bool
+    (requires fun h -> True)  
+    (ensures fun h0 _ h1 -> True)
+
+
+let ecdsa_verification pubKey r s mLen m tempBuffer = 
+    (*check that publicKey is not equal to the identity element O *)
+  (*let pointInfinityPublicKey = isPointAtInfinity pubKey in 
+    if pointInfinityPublicKey = true then false else *)
+  let coordinatesValid = isCoordinateValid pubKey in
+    if coordinatesValid = true then false else 
+  let belongsToCurve =  isPointOnCurve pubKey in 
+    if belongsToCurve = false then false else true
